stubs/pickle_stubs_secure/__init__.pyi
@@ -1,4 +1,5 @@
 from pickle_stubs_secure._unsafe import Unsafe as Unsafe
 from pickle_stubs_secure.trust import TrustedArtifact as TrustedArtifact
 from pickle_stubs_secure.trust import TrustedBytes as TrustedBytes
+from pickle_stubs_secure.trust import TrustedBinaryIO as TrustedBinaryIO
 from pickle_stubs_secure.trust import TrustedPath as TrustedPath
